PAC_Checker2/LPAC_Checker_Specification.thy
@@ -5,7 +5,7 @@
 *)
 theory LPAC_Checker_Specification
   imports LPAC_Specification
-    Refine_Imperative_HOL.IICF
+    Isabelle_LLVM.IICF
     PAC_Checker.Finite_Map_Multiset
     PAC_Checker.PAC_Checker_Specification
 begin
